\item 
\begin{enumerate}
    \item \begin{answer}
        \begin{align*}
            A &= T\Lambda T^{-1} \\
            AT &= T\Lambda \\
            A \begin{bmatrix}
                t^{(1)} & \cdots & t^{(n)}
            \end{bmatrix} &= 
            \begin{bmatrix}
                t^{(1)} & \cdots & t^{(n)}
            \end{bmatrix}
            \begin{bmatrix}
                \lambda_1 & 0 & \cdots & 0 \\
                0 & \lambda_2 & \cdots & 0 \\
                \vdots & \vdots & \ddots & \vdots \\
                0 & 0 & \cdots & \lambda_n
            \end{bmatrix} \\
            \begin{bmatrix}
                At^{(1)} & \cdots & At^{(n)}
            \end{bmatrix} &= 
            \begin{bmatrix}
                \lambda_1 t^{(1)} & \cdots & \lambda_n t^{(n)}
            \end{bmatrix}
        \end{align*}
        Therefore, we have: $At^{(i)} = \lambda_i t^{(i)}$.
    \end{answer}

    \item \begin{answer}
        \begin{align*}
            A &= U\Lambda U^{\top} \\
            AU &= U\Lambda \\
            A \begin{bmatrix}
                u^{(1)} & \cdots & u^{(n)}
            \end{bmatrix} &= 
            \begin{bmatrix}
                u^{(1)} & \cdots & u^{(n)}
            \end{bmatrix}
            \begin{bmatrix}
                \lambda_1 & 0 & \cdots & 0 \\
                0 & \lambda_2 & \cdots & 0 \\
                \vdots & \vdots & \ddots & \vdots \\
                0 & 0 & \cdots & \lambda_n
            \end{bmatrix} \\
            \begin{bmatrix}
                Au^{(1)} & \cdots & Au^{(n)}
            \end{bmatrix} &= 
            \begin{bmatrix}
                \lambda_1 u^{(1)} & \cdots & \lambda_n u^{(n)}
            \end{bmatrix}
        \end{align*}
        Therefore, we have: $Au^{(i)} = \lambda_i u^{(i)}$.
    \end{answer}

    \item \begin{answer}
        From part (b), $Au^{(i)} = \lambda_i u^{(i)}$.
        $$(u^{(i)})^{\top}Au^{(i)} = (u^{(i)})^{\top}\lambda_i u^{(i)} = \lambda_i (u^{(i)})^{\top} u^{(i)} = \lambda_i \ge 0$$
    \end{answer}
\end{enumerate}